remove refinement for module Lock_DistributedSystem_i

ironfleet/src/Dafny/Distributed/Services/Lock/LockDistributedSystem.i.dfy
@@ -1,8 +1,66 @@
 include "../../Impl/Lock/Host.i.dfy"
 include "../../Common/Framework/DistributedSystem.s.dfy"
 
-module Lock_DistributedSystem_i refines DistributedSystem_s {
 
-    import H_s = Host_i`All
+// Remove refinement for Dafny 4.2.0
+// module Lock_DistributedSystem_i refines DistributedSystem_s {
+module Lock_DistributedSystem_i {
+    // import opened H_s = Host_s
+    import opened Collections__Maps2_s
+    import opened Native__Io_s
+    import opened Environment_s
+    import opened Native__NativeTypes_s
+
+    import opened H_s = Host_i`All
+
+    /////////////////////////////////////////
+    // PHYSICAL ENVIRONMENT
+    /////////////////////////////////////////
+
+    ghost predicate ValidPhysicalEnvironmentStep(step:LEnvStep<EndPoint, seq<byte>>)
+    {
+    step.LEnvStepHostIos? ==> forall io{:trigger io in step.ios}{:trigger ValidPhysicalIo(io)} :: io in step.ios ==> ValidPhysicalIo(io)
+    }
+
+    /////////////////////////////////////////
+    // DS_State
+    /////////////////////////////////////////
+
+    datatype DS_State = DS_State(
+        config:H_s.ConcreteConfiguration,
+        environment:LEnvironment<EndPoint,seq<byte>>,
+        servers:map<EndPoint,H_s.HostState>
+    )
+
+    ghost predicate DS_Init(s:DS_State, config:H_s.ConcreteConfiguration)
+    reads *
+    {
+        && s.config == config
+        && H_s.ConcreteConfigToServers(s.config) == mapdomain(s.servers)
+        && H_s.ConcreteConfigInit(s.config)
+        && LEnvironment_Init(s.environment)
+        && (forall id :: id in s.servers ==> H_s.HostInit(s.servers[id], config, id))
+    }
+    
+    ghost predicate DS_NextOneServer(s:DS_State, s':DS_State, id:EndPoint, ios:seq<LIoOp<EndPoint,seq<byte>>>)
+    requires id in s.servers
+    reads *
+    {
+        && id in s'.servers
+        && H_s.HostNext(s.servers[id], s'.servers[id], ios)
+        && s'.servers == s.servers[id := s'.servers[id]]
+    }
+
+    ghost predicate DS_Next(s:DS_State, s':DS_State)
+    reads *
+    {
+        && s'.config == s.config
+        && LEnvironment_Next(s.environment, s'.environment)
+        && ValidPhysicalEnvironmentStep(s.environment.nextStep)
+        && if s.environment.nextStep.LEnvStepHostIos? && s.environment.nextStep.actor in s.servers then
+            DS_NextOneServer(s, s', s.environment.nextStep.actor, s.environment.nextStep.ios)
+            else
+            s'.servers == s.servers
+    }
 
 }
